platform/tests/ListBuilder.v
@@ -8,10 +8,10 @@ Module T := Thread0.Make(M).
 Import T.
 
 Definition handlerS := SPEC reserving 29
-  PREonly[_] sched * mallocHeap 0.
+  PREmain[_] sched * mallocHeap 0.
 
-Definition mainS := SPEC reserving 36
-  PREonly[_] globalSched =?> 1 * mallocHeap 0.
+Definition mainS := SPEC reserving 49
+  PREmain[_] globalSched =?> 1 * mallocHeap 0.
 
 Definition m := bimport [[ "malloc"!"malloc" @ [mallocS], "malloc"!"free" @ [freeS],
                            "scheduler"!"init" @ [initS], "scheduler"!"exit" @ [exitS],
@@ -21,10 +21,10 @@ Definition m := bimport [[ "malloc"!"malloc" @ [mallocS], "malloc"!"free" @ [fre
       "i" <- 0;; (* Loop counter *)
       "p" <- 0;; (* Pointer to head of list we will build *)
 
-      [PREonly[V] Ex ls, sll ls (V "p") * sched * mallocHeap 0]
+      [PREmain[V] Ex ls, sll ls (V "p") * sched * mallocHeap 0]
       While ("i" < 10) {
         "r" <-- Call "malloc"!"malloc"(0, 2)
-        [PREonly[V, R] [| R <> 0 |] * [| freeable R 2 |] * R =?> 2 * Ex ls, sll ls (V "p") * sched * mallocHeap 0];;
+        [PREmain[V, R] [| R <> 0 |] * [| freeable R 2 |] * R =?> 2 * Ex ls, sll ls (V "p") * sched * mallocHeap 0];;
 
         "r" *<- "i";;
         "r" + 4 *<- "p";;
@@ -32,37 +32,37 @@ Definition m := bimport [[ "malloc"!"malloc" @ [mallocS], "malloc"!"free" @ [fre
         "i" <- "i" + 1;;
 
         Yield
-        [PREonly[V] Ex ls, sll ls (V "p") * sched * mallocHeap 0]
+        [PREmain[V] Ex ls, sll ls (V "p") * sched * mallocHeap 0]
       };;
 
-      [PREonly[V] Ex ls, sll ls (V "p") * sched * mallocHeap 0]
+      [PREmain[V] Ex ls, sll ls (V "p") * sched * mallocHeap 0]
       While ("p" <> 0) {
         "r" <- "p";;
         "p" <-* "p" + 4;;
         Call "malloc"!"free"(0, "r", 2)
-        [PREonly[V] Ex ls, sll ls (V "p") * sched * mallocHeap 0];;
+        [PREmain[V] Ex ls, sll ls (V "p") * sched * mallocHeap 0];;
 
         Yield
-        [PREonly[V] Ex ls, sll ls (V "p") * sched * mallocHeap 0]
+        [PREmain[V] Ex ls, sll ls (V "p") * sched * mallocHeap 0]
       };;
 
-      Exit
-    end with bfunctionNoRet "main"("sc") [mainS]
+      Exit 30
+    end with bfunctionNoRet "main"("x", "y") [mainS]
       Init
-      [PREonly[_] sched * mallocHeap 0];;
+      [PREmain[_] sched * mallocHeap 0];;
 
       Spawn("test"!"handler", 30)
-      [PREonly[_] sched * mallocHeap 0];;
+      [PREmain[_] sched * mallocHeap 0];;
 
       Spawn("test"!"handler", 30)
-      [PREonly[_] sched * mallocHeap 0];;
+      [PREmain[_] sched * mallocHeap 0];;
 
-      Go
+      Go 50
     end
   }}.
 
 Theorem ok : moduleOk m.
-  vcgen; abstract sep SinglyLinkedList.hints.
+  vcgen; abstract (sep SinglyLinkedList.hints; auto).
 Qed.
 
 End Make.
