platform/tests/Yield.v
@@ -8,31 +8,31 @@ Module T := Thread0.Make(M).
 Import T.
 
 Definition handlerS := SPEC reserving 26
-  PREonly[_] sched * mallocHeap 0.
+  PREmain[_] sched * mallocHeap 0.
 
-Definition mainS := SPEC reserving 36
-  PREonly[_] M.globalSched =?> 1 * mallocHeap 0.
+Definition mainS := SPEC reserving 49
+  PREmain[_] M.globalSched =?> 1 * mallocHeap 0.
 
 Definition m := bimport [[ "scheduler"!"init" @ [initS], "scheduler"!"exit" @ [exitS],
                            "scheduler"!"spawn" @ [spawnS], "scheduler"!"yield" @ [yieldS] ]]
   bmodule "test" {{
-    bfunctionNoRet "handler"() [handlerS]
+    bfunctionNoRet "handler"("x", "y") [handlerS]
       Yield
-      [PREonly[_] sched * mallocHeap 0];;
-      Exit
-    end with bfunctionNoRet "main"() [mainS]
+      [PREmain[_] sched * mallocHeap 0];;
+      Exit 27
+    end with bfunctionNoRet "main"("x", "y") [mainS]
       Init
-      [PREonly[_] sched * mallocHeap 0];;
+      [PREmain[_] sched * mallocHeap 0];;
 
       Spawn("test"!"handler", 27)
-      [PREonly[_] sched * mallocHeap 0];;
+      [PREmain[_] sched * mallocHeap 0];;
 
-      Go
+      Go 50
     end
   }}.
 
 Theorem ok : moduleOk m.
-  vcgen; abstract sep_auto.
+  vcgen; abstract (sep_auto; auto).
 Qed.
 
 End Make.
